use new res_step'_separate_e, remove unused func

theories/interpreter_func.v
@@ -82,10 +82,10 @@ Inductive res_step'_separate_e
   (hs : host_state) (s : store_record) (f : frame)
   (ves : list value) (e : administrative_instruction) : Type :=
 | RS''_exhaustion : res_step'_separate_e hs s f ves e
-| RS''_error (inst : instance) :
+| RS''_error :
     (~ exists C ts1 ts2 ts1',
       map typeof ves = ts1' ++ ts1 /\
-      inst_typing s inst C /\
+      inst_typing s f.(f_inst) C /\
       e_typing s C ((vs_to_es ves) ++ [::e]) (Tf ts1 ts2)) ->
     res_step'_separate_e hs s f ves e
 (* | RS''_break *)
@@ -98,6 +98,7 @@ Inductive res_step'_separate_e
  * stated. Their values could be inferred from the type of H instead but we
  * want to make those values clear. *)
 Notation "<< hs' , s' , f' , es' >>[ H ]" := (@RS'_normal _ _ _ _ hs' s' f' es' H).
+Notation "<< hs' , s' , f' , es' >>'[ H ]" := (@RS''_normal _ _ _ _ _ hs' s' f' es' H).
 
 (* Using this as a TODO placeholder *)
 Axiom admitted_TODO : forall P : Prop, P.
@@ -137,7 +138,8 @@ Definition config_tuple_separate_e_typing (cfg : config_one_tuple_without_e) (e 
 Definition res_tuple := (host_state * store_record * frame * res_step)%type.
 
 (* TODO *)
-Axiom coerce_res : forall hs s f es1 es2 (r : res_step' hs s f es1), res_step' hs s f es2.
+Axiom coerce_res : forall hs s f es ves e (r : res_step'_separate_e hs s f ves e),
+  res_step' hs s f es.
 
 (* TODO auto instantiate lh, k? *)
 (* TODO better name *)
@@ -145,11 +147,12 @@ Ltac solve_lfilled_0 :=
   unfold lfilled, lfill, vs_to_es;
   try rewrite v_to_e_is_const_list; apply/eqP; simplify_lists => //.
 
-Lemma reduce_unop : forall (hs : host_state) s f t op v ves' es0,
-  es0 = vs_to_es (v :: ves') ++ [:: AI_basic (BI_unop t op)] ->
-  reduce hs s f es0 hs s f (vs_to_es (app_unop op v :: ves')).
+Lemma reduce_unop : forall (hs : host_state) s f t op v ves',
+  reduce
+    hs s f (vs_to_es (v :: ves') ++ [:: AI_basic (BI_unop t op)])
+    hs s f (vs_to_es (app_unop op v :: ves')).
 Proof.
-  intros hs s f t op v ves' es0 ?. subst es0.
+  intros hs s f t op v ves'.
   eapply r_label with (k := 0) (lh := (LH_base (vs_to_es ves') [::])).
   - apply r_simple. by apply rs_unop.
   - by solve_lfilled_0.
@@ -206,7 +209,8 @@ Proof.
   - assert (es = [::]).
     { destruct es => //. apply extract_list1 in H2 as [H?]. discriminate H. }
     subst es.
-    assert (e = AI_basic (BI_unop t op)). { simpl in H2. by inversion H2. } subst e.
+    assert (e = AI_basic (BI_unop t op)). { simpl in H2. by inversion H2. }
+    subst e.
     symmetry in H3. apply cat0_inv in H3 as [??]. subst t1s' t1s0.
     assert (t2s = [::]). { by apply empty_e_typing in Hetype1. } subst t2s.
     eapply IHHetype2 => //. by assumption.
@@ -215,12 +219,13 @@ Proof.
     eapply IHHetype => //. by assumption.
 Qed.
 
-Lemma reduce_binop : forall (hs : host_state) s f t op v1 v2 v ves' es0,
-  es0 = vs_to_es [:: v2, v1 & ves'] ++ [:: AI_basic (BI_binop t op)] ->
+Lemma reduce_binop : forall (hs : host_state) s f t op v1 v2 v ves',
   app_binop op v1 v2 = Some v ->
-  reduce hs s f es0 hs s f (vs_to_es (v :: ves')).
+  reduce
+    hs s f (vs_to_es [:: v2, v1 & ves'] ++ [:: AI_basic (BI_binop t op)])
+    hs s f (vs_to_es (v :: ves')).
 Proof.
-  intros hs s f t op v1 v2 v ves' es0 ? Heqapp. subst es0.
+  intros hs s f t op v1 v2 v ves' Heqapp.
   eapply r_label with (k := 0) (lh := (LH_base (vs_to_es ves') [::])).
   - apply r_simple.
     apply rs_binop_success.
@@ -269,382 +274,8 @@ Admitted.
     * give_up.
    *)
 
-Fixpoint run_step_with_fuel' hs s f es (fuel : fuel) (d : depth) : res_step' hs s f es :=
-  match fuel with
-  | 0 => RS'_exhaustion hs s f es
-  | fuel.+1 =>
-    let: (ves, es') := split_vals_e es in (** Framing out constants. **)
-    match es' with
-    | [::] => RS'_error _ _ (admitted_TODO (~ exists C t, e_typing s C es t))
-    | e :: es'' =>
-      if e_is_trap e
-      then
-        if (es'' != [::]) || (ves != [::])
-        then RS'_normal (admitted_TODO (reduce hs s f es hs s f [::AI_trap]))
-        else RS'_error hs f (admitted_TODO (~ exists C t, e_typing s C es t))      else
-        let: cfg'             := (hs, s, f, (rev ves)) in
-        (* TODO: this will need some proof of (es = (rev ves) ++ [::e] ++ es'')
-         * or similar, not sure how that will work*)
-        let: r := run_one_step' hs s f ves e fuel d in
-        if r is RS'_normal hs' s' f' es' _ (* TODO *)
-        then RS'_normal (admitted_TODO (reduce hs s f es hs' s' f' (es' ++ es'')))
-        else coerce_res _ r (* TODO *)
-    end
-  end
-
-with run_one_step' hs s f ves e (fuel : fuel) (d : depth) : res_step' hs s f ((vs_to_es ves) ++ [::e]) :=
-  let: es0 := (vs_to_es ves) ++ [::e] in (* initial es, useful as an arg for reduce *)
-  match fuel with
-  | 0 => RS'_exhaustion _ _ _ _
-  | fuel.+1 =>
-    match e with
-    (* unop *)
-    | AI_basic (BI_unop t op) =>
-      if ves is v :: ves'
-      then <<hs, s, f, vs_to_es (app_unop op v :: ves')>>[ admitted_TODO _ ]
-      else RS'_error _ _ (admitted_TODO _)
-    (* binop *)
-    | AI_basic (BI_binop t op) =>
-      if ves is v2 :: v1 :: ves' then
-        let vo := app_binop op v1 v2 in
-        match vo with
-        | Some v => <<hs, s, f, vs_to_es (v :: ves')>>[ admitted_TODO _ ]
-        | None => RS'_error _ _ (admitted_TODO _)
-        end
-      else RS'_error _ _ (admitted_TODO _)
-    (* testops *)
-    | AI_basic (BI_testop T_i32 testop) =>
-      if ves is (VAL_int32 c) :: ves' then
-        RS'_normal (admitted_TODO
-              (reduce hs s f es0 hs s f (vs_to_es ((VAL_int32 (wasm_bool (@app_testop_i i32t testop c))) :: ves'))))
-      else RS'_error _ _ (admitted_TODO _)
-    | AI_basic (BI_testop T_i64 testop) =>
-      if ves is (VAL_int64 c) :: ves' then
-        RS'_normal (admitted_TODO
-              (reduce hs s f es0 hs s f (vs_to_es ((VAL_int32 (wasm_bool (@app_testop_i i64t testop c))) :: ves'))))
-      else RS'_error _ _ (admitted_TODO _)
-    | AI_basic (BI_testop _ _) => RS'_error _ _ (admitted_TODO _)
-    (* relops *)
-    | AI_basic (BI_relop t op) =>
-      if ves is v2 :: v1 :: ves' then
-        RS'_normal (admitted_TODO
-              (reduce hs s f es0 hs s f (vs_to_es (VAL_int32 (wasm_bool (app_relop op v1 v2)) :: ves'))))
-      else RS'_error _ _ (admitted_TODO _)
-    (* convert & reinterpret *)
-    | AI_basic (BI_cvtop t2 CVO_convert t1 sx) =>
-      if ves is v :: ves' then
-        if types_agree t1 v
-        then
-          expect (cvt t2 sx v) (fun v' =>
-               RS'_normal (admitted_TODO
-               (reduce hs s f es0 hs s f (vs_to_es (v' :: ves')))))
-               (RS'_normal (admitted_TODO
-               (reduce hs s f es0 hs s f ((vs_to_es ves') ++ [::AI_trap]))))
-        else RS'_error _ _ (admitted_TODO _)
-      else RS'_error _ _ (admitted_TODO _)
-    | AI_basic (BI_cvtop t2 CVO_reinterpret t1 sx) =>
-      if ves is v :: ves' then
-        if types_agree t1 v && (sx == None)
-        then RS'_normal (admitted_TODO
-              (reduce hs s f es0 hs s f (vs_to_es (wasm_deserialise (bits v) t2 :: ves'))))
-        else RS'_error _ _ (admitted_TODO _)
-      else RS'_error _ _ (admitted_TODO _)
-    (**)
-    | AI_basic BI_unreachable => RS'_normal
-        (admitted_TODO (reduce hs s f es0 hs s f ((vs_to_es ves) ++ [::AI_trap])))
-    | AI_basic BI_nop => RS'_normal
-        (admitted_TODO (reduce hs s f es0 hs s f (vs_to_es ves)))
-    | AI_basic BI_drop =>
-      if ves is v :: ves' then
-        RS'_normal (admitted_TODO (reduce hs s f es0 hs s f (vs_to_es ves')))
-      else RS'_error _ _ (admitted_TODO _)
-    | AI_basic BI_select =>
-      if ves is (VAL_int32 c) :: v2 :: v1 :: ves' then
-        if c == Wasm_int.int_zero i32m
-        then RS'_normal (admitted_TODO
-          (reduce hs s f es0 hs s f (vs_to_es (v2 :: ves'))))
-        else RS'_normal (admitted_TODO
-          (reduce hs s f es0 hs s f (vs_to_es (v1 :: ves'))))
-      else RS'_error _ _ (admitted_TODO _)
-    | AI_basic (BI_block (Tf t1s t2s) es) =>
-      if length ves >= length t1s
-      then
-        let: (ves', ves'')  := split_n ves (length t1s) in
-        RS'_normal (admitted_TODO
-          (reduce hs s f es0 hs s f
-            (vs_to_es ves'' ++ [::AI_label (length t2s) [::] (vs_to_es ves' ++ to_e_list es)])
-        ))
-      else RS'_error _ _ (admitted_TODO _)
-    | AI_basic (BI_loop (Tf t1s t2s) es) =>
-      if length ves >= length t1s
-      then
-        let: (ves', ves'') := split_n ves (length t1s) in
-        RS'_normal (admitted_TODO
-          (reduce hs s f es0 hs s f
-            (vs_to_es ves''
-                    ++ [::AI_label (length t1s) [::AI_basic (BI_loop (Tf t1s t2s) es)]
-                            (vs_to_es ves' ++ to_e_list es)])
-        ))
-      else RS'_error _ _ (admitted_TODO _)
-    | AI_basic (BI_if tf es1 es2) =>
-      if ves is VAL_int32 c :: ves' then
-        if c == Wasm_int.int_zero i32m
-        then RS'_normal (admitted_TODO
-        (reduce hs s f es0 hs s f (vs_to_es ves' ++ [::AI_basic (BI_block tf es2)])))
-        else RS'_normal (admitted_TODO 
-        (reduce hs s f es0 hs s f (vs_to_es ves' ++ [::AI_basic (BI_block tf es1)])))
-      else RS'_error _ _ (admitted_TODO _)
-    | AI_basic (BI_br j) => RS'_break _ _ _ _ hs s f j ves
-    | AI_basic (BI_br_if j) =>
-      if ves is VAL_int32 c :: ves' then
-        if c == Wasm_int.int_zero i32m
-        then RS'_normal (admitted_TODO
-        (reduce hs s f es0 hs s f (vs_to_es ves')))
-        else RS'_normal (admitted_TODO
-        (reduce hs s f es0 hs s f (vs_to_es ves' ++ [::AI_basic (BI_br j)])))
-      else RS'_error _ _ (admitted_TODO _)
-    | AI_basic (BI_br_table js j) =>
-      if ves is VAL_int32 c :: ves' then
-        let: k := Wasm_int.nat_of_uint i32m c in
-        if k < length js
-        then
-          expect (List.nth_error js k) (fun js_at_k =>
-              RS'_normal (admitted_TODO
-                (reduce hs s f es0 hs s f (vs_to_es ves' ++ [::AI_basic (BI_br js_at_k)]))))
-            (RS'_error _ _ (admitted_TODO _))
-        else RS'_normal (admitted_TODO
-               (reduce hs s f es0 hs s f (vs_to_es ves' ++ [::AI_basic (BI_br j)])))
-      else RS'_error _ _ (admitted_TODO _)
-    | AI_basic (BI_call j) =>
-      if List.nth_error f.(f_inst).(inst_funcs) j is Some a then
-        RS'_normal (admitted_TODO
-          (reduce hs s f es0 hs s f (vs_to_es ves ++ [::AI_invoke a])))
-      else RS'_error _ _ (admitted_TODO _)
-    | AI_basic (BI_call_indirect j) =>
-      if ves is VAL_int32 c :: ves' then
-        match stab_addr s f (Wasm_int.nat_of_uint i32m c) with
-        | Some a =>
-          match List.nth_error s.(s_funcs) a with
-          | Some cl =>
-            if stypes s f.(f_inst) j == Some (cl_type cl)
-            then RS'_normal (admitted_TODO
-              (reduce hs s f es0 hs s f (vs_to_es ves' ++ [::AI_invoke a])))
-            else RS'_normal (admitted_TODO
-              (reduce hs s f es0 hs s f (vs_to_es ves' ++ [::AI_trap])))
-          | None => RS'_error _ _ (admitted_TODO _)
-          end
-        | None => RS'_normal (admitted_TODO
-              (reduce hs s f es0 hs s f (vs_to_es ves' ++ [::AI_trap])))
-        end
-      else RS'_error _ _ (admitted_TODO _)
-    | AI_basic BI_return => RS'_return _ _ _ _ hs s f ves
-    | AI_basic (BI_get_local j) =>
-      if j < length f.(f_locs)
-      then
-        expect (List.nth_error f.(f_locs) j) (fun vs_at_j =>
-            RS'_normal (admitted_TODO
-              (reduce hs s f es0 hs s f (vs_to_es (vs_at_j :: ves)))))
-          (RS'_error _ _ (admitted_TODO _))
-      else RS'_error _ _ (admitted_TODO _)
-    | AI_basic (BI_set_local j) =>
-      if ves is v :: ves' then
-        if j < length f.(f_locs)
-        then
-          let f' := Build_frame (update_list_at f.(f_locs) j v) f.(f_inst) in
-          RS'_normal (admitted_TODO
-            (reduce hs s f es0 hs s f' (vs_to_es ves')))
-        else RS'_error _ _ (admitted_TODO _)
-      else RS'_error _ _ (admitted_TODO _)
-    | AI_basic (BI_tee_local j) =>
-      if ves is v :: ves' then
-        RS'_normal (admitted_TODO
-              (reduce hs s f es0 hs s f (vs_to_es (v :: ves) ++ [::AI_basic (BI_set_local j)])))
-      else RS'_error _ _ (admitted_TODO _)
-    | AI_basic (BI_get_global j) =>
-      if sglob_val s f.(f_inst) j is Some xx
-      then RS'_normal (admitted_TODO
-              (reduce hs s f es0 hs s f (vs_to_es (xx :: ves))))
-      else RS'_error _ _ (admitted_TODO _)
-    | AI_basic (BI_set_global j) =>
-      if ves is v :: ves' then
-        if supdate_glob s f.(f_inst) j v is Some xx
-        then RS'_normal (admitted_TODO
-              (reduce hs s f es0 hs s f (vs_to_es ves')))
-        else RS'_error _ _ (admitted_TODO _)
-      else RS'_error _ _ (admitted_TODO _)
-    | AI_basic (BI_load t None a off) =>
-      if ves is VAL_int32 k :: ves' then
-        expect
-          (smem_ind s f.(f_inst))
-          (fun j =>
-             if List.nth_error s.(s_mems) j is Some mem_s_j then
-               expect
-                 (load (mem_s_j) (Wasm_int.N_of_uint i32m k) off (t_length t))
-                 (fun bs => RS'_normal (admitted_TODO (reduce hs s f es0 hs s f (vs_to_es (wasm_deserialise bs t :: ves')))))
-                 (RS'_normal (admitted_TODO (reduce hs s f es0 hs s f (vs_to_es ves' ++ [::AI_trap]))))
-             else RS'_error _ _ (admitted_TODO _))
-          (RS'_error _ _ (admitted_TODO _))
-      else RS'_error _ _ (admitted_TODO _)
-    | AI_basic (BI_load t (Some (tp, sx)) a off) =>
-      if ves is VAL_int32 k :: ves' then
-        expect
-          (smem_ind s f.(f_inst))
-          (fun j =>
-             if List.nth_error s.(s_mems) j is Some mem_s_j then
-               expect
-                 (load_packed sx (mem_s_j) (Wasm_int.N_of_uint i32m k) off (tp_length tp) (t_length t))
-                 (fun bs => RS'_normal (admitted_TODO (reduce hs s f es0 hs s f (vs_to_es (wasm_deserialise bs t :: ves')))))
-                 (RS'_normal (admitted_TODO (reduce hs s f es0 hs s f (vs_to_es ves' ++ [::AI_trap]))))
-             else RS'_error _ _ (admitted_TODO _))
-          (RS'_error _ _ (admitted_TODO _))
-      else RS'_error _ _ (admitted_TODO _)
-    | AI_basic (BI_store t None a off) =>
-      if ves is v :: VAL_int32 k :: ves' then
-        if types_agree t v
-        then
-          expect
-            (smem_ind s f.(f_inst))
-            (fun j =>
-               if List.nth_error s.(s_mems) j is Some mem_s_j then
-                 expect
-                   (store mem_s_j (Wasm_int.N_of_uint i32m k) off (bits v) (t_length t))
-                   (fun mem' =>
-                      let s' := upd_s_mem s (update_list_at s.(s_mems) j mem') in
-                      (RS'_normal (admitted_TODO (reduce hs s f es0 hs s f (vs_to_es ves')))))
-                   (RS'_normal (admitted_TODO (reduce hs s f es0 hs s f (vs_to_es ves' ++ [::AI_trap]))))
-               else RS'_error _ _ (admitted_TODO _))
-            (RS'_error _ _ (admitted_TODO _))
-        else RS'_error _ _ (admitted_TODO _)
-      else RS'_error _ _ (admitted_TODO _)
-    | AI_basic (BI_store t (Some tp) a off) =>
-      if ves is v :: VAL_int32 k :: ves' then
-        if types_agree t v
-        then
-          expect
-            (smem_ind s f.(f_inst))
-            (fun j =>
-               if List.nth_error s.(s_mems) j is Some mem_s_j then
-                 expect
-                   (store_packed mem_s_j (Wasm_int.N_of_uint i32m k) off (bits v) (tp_length tp))
-                   (fun mem' =>
-                      let s' := upd_s_mem s (update_list_at s.(s_mems) j mem') in
-                      (RS'_normal (admitted_TODO (reduce hs s f es0 hs s' f (vs_to_es ves')))))
-                   (RS'_normal (admitted_TODO (reduce hs s f es0 hs s f (vs_to_es ves' ++ [::AI_trap]))))
-               else RS'_error _ _ (admitted_TODO _))
-            (RS'_error _ _ (admitted_TODO _))
-        else RS'_error _ _ (admitted_TODO _)
-      else RS'_error _ _ (admitted_TODO _)
-    | AI_basic BI_current_memory =>
-      expect
-        (smem_ind s f.(f_inst))
-        (fun j =>
-           if List.nth_error s.(s_mems) j is Some s_mem_s_j then
-             RS'_normal
-             (admitted_TODO (reduce hs s f es0 hs s f (vs_to_es (VAL_int32 (Wasm_int.int_of_Z i32m (Z.of_nat (mem_size s_mem_s_j))) :: ves))))
-           else RS'_error _ _ (admitted_TODO _))
-        (RS'_error _ _ (admitted_TODO _))
-    | AI_basic BI_grow_memory =>
-      if ves is VAL_int32 c :: ves' then
-        expect
-          (smem_ind s f.(f_inst))
-          (fun j =>
-            if List.nth_error s.(s_mems) j is Some s_mem_s_j then
-              let: l := mem_size s_mem_s_j in
-              let: mem' := mem_grow s_mem_s_j (Wasm_int.N_of_uint i32m c) in
-              if mem' is Some mem'' then
-                let s' := upd_s_mem s (update_list_at s.(s_mems) j mem'') in
-                RS'_normal (admitted_TODO
-                 (reduce hs s f es0 hs s' f (vs_to_es (VAL_int32 (Wasm_int.int_of_Z i32m (Z.of_nat l)) :: ves'))))
-              else RS'_error _ _ (admitted_TODO _)
-            else RS'_error _ _ (admitted_TODO _))
-          (RS'_error _ _ (admitted_TODO _))
-      else RS'_error _ _ (admitted_TODO _)
-    | AI_basic (BI_const _) => RS'_error _ _ (admitted_TODO _)
-    | AI_invoke a =>
-      match List.nth_error s.(s_funcs) a with
-      | Some cl => 
-        match cl with
-        | FC_func_native i (Tf t1s t2s) ts es =>
-            let: n := length t1s in
-            let: m := length t2s in
-            if length ves >= n
-            then
-            let: (ves', ves'') := split_n ves n in
-            let: zs := n_zeros ts in
-            RS'_normal (admitted_TODO (reduce hs s f es0 hs s f
-              (vs_to_es ves'' ++ [::AI_local m (Build_frame (rev ves' ++ zs) i) [::AI_basic (BI_block (Tf [::] t2s) es)]])))
-            else RS'_error _ _ (admitted_TODO _)
-        | FC_func_host (Tf t1s t2s) cl' =>
-            let: n := length t1s in
-            let: m := length t2s in
-            if length ves >= n
-            then
-            let: (ves', ves'') := split_n ves n in
-            match host_application_impl hs s (Tf t1s t2s) cl' (rev ves') with
-            | (hs', Some (s', rves)) =>
-                RS'_normal (admitted_TODO
-                  (reduce hs s f es0 hs' s' f (vs_to_es ves'' ++ (result_to_stack rves))))
-            | (hs', None) => RS'_normal (admitted_TODO
-                (reduce hs s f es0 hs' s f (vs_to_es ves ++ [::AI_invoke a])))
-            end
-            else RS'_error _ _ (admitted_TODO _)
-        end
-      | None => RS'_error _ _ (admitted_TODO _)
-      end
-    | AI_label ln les es =>
-      if es_is_trap es
-      then RS'_normal (admitted_TODO
-              (reduce hs s f es0 hs s f (vs_to_es ves ++ [::AI_trap])))
-      else
-        if const_list es
-        then RS'_normal (admitted_TODO
-              (reduce hs s f es0 hs s f (vs_to_es ves ++ es)))
-        else
-          match run_step_with_fuel' hs s f es fuel d with
-          | RS'_break hs' s' f' 0 bvs =>
-            if length bvs >= ln
-            then RS'_normal (admitted_TODO
-              (reduce hs s f es0 hs' s' f' ((vs_to_es ((take ln bvs) ++ ves)) ++ les)))
-            else RS'_error _ _ (admitted_TODO _)
-          | RS'_break hs' s' f' (n.+1) bvs => RS'_break _ _ _ _ hs' s' f' n bvs
-          | RS'_return hs' s' f' rvs => RS'_return _ _ _ _ hs' s' f' rvs
-          | RS'_normal hs' s' f' es' _ =>
-            RS'_normal (admitted_TODO
-              (reduce hs s f es0 hs' s' f' (vs_to_es ves ++ [::AI_label ln les es'])))
-          | RS'_error _ => RS'_error _ _ (admitted_TODO _)
-          | RS'_exhaustion => RS'_exhaustion _ _ _ _
-          end
-    | AI_local ln lf es =>
-      if es_is_trap es
-      then RS'_normal (admitted_TODO
-              (reduce hs s f es0 hs s f (vs_to_es ves ++ [::AI_trap])))
-      else
-        if const_list es
-        then
-          if length es == ln
-          then RS'_normal (admitted_TODO
-                 (reduce hs s f es0 hs s f (vs_to_es ves ++ es)))
-          else RS'_error _ _ (admitted_TODO _)
-        else
-          match run_step_with_fuel' hs s f es fuel d with
-          | RS'_return hs' s' f' rvs =>
-            if length rvs >= ln
-            then RS'_normal (admitted_TODO
-              (reduce hs s f es0 hs' s' f (vs_to_es (take ln rvs ++ ves))))
-            else RS'_error _ _ (admitted_TODO _)
-          | RS'_normal hs' s' f' es' _ =>
-            RS'_normal (admitted_TODO
-              (reduce hs s f es0 hs' s' f (vs_to_es ves ++ [::AI_local ln f' es'])))
-          | RS'_error _ => RS'_error _ _ (admitted_TODO _)
-          | RS'_exhaustion => RS'_exhaustion _ _ _ _
-          | RS'_break _ _ _ _ _ => RS'_error _ _ (admitted_TODO _)
-          end
-    | AI_trap => RS'_error _ _ (admitted_TODO _)
-    end
-  end.
-
 Theorem run_step_with_fuel'' hs s f es (fuel : fuel) (d : depth) : res_step' hs s f es
-with run_one_step'' hs s f ves e (fuel : fuel) (d : depth) : res_step' hs s f ((vs_to_es ves) ++ [::e]).
+with run_one_step'' hs s f ves e (fuel : fuel) (d : depth) : res_step'_separate_e hs s f ves e.
 (* TODO should use res_step'_separate_e *)
 Proof.
   (* NOTE: not indenting the two main subgoals *)
@@ -664,7 +295,7 @@ Proof.
         -- apply <<hs, s, f, [::AI_trap]>>[admitted_TODO _].
         -- apply (RS'_error _ _ (admitted_TODO (~ exists C t, e_typing s C es t))).
       + remember (run_one_step'' hs s f (rev ves) e fuel d) as r.
-        apply (if r is RS'_normal hs' s' f' es' _
+        apply (if r is RS''_normal hs' s' f' es' _
           then <<hs', s', f', (es' ++ es'')>>[admitted_TODO _]
           else coerce_res _ r).
 
@@ -673,7 +304,7 @@ Proof.
   remember ((vs_to_es ves) ++ [::e]) as es0 eqn:Heqes0.
   destruct fuel as [|fuel].
   - (* 0 *)
-    apply RS'_exhaustion.
+    apply RS''_exhaustion.
   - (* fuel.+1 *)
     destruct e as [
       (* AI_basic *) [
@@ -763,29 +394,26 @@ Proof.
     * (* AI_basic (BI_unop t op) *)
       destruct ves as [|v ves'] eqn:Heqves.
       + (* [::] *)
-        assert (inst : instance). { give_up. (* TODO need an instance *) }
-        (* TODO need to change return type to be able to apply RS''_error *)
-        Check (@RS''_error hs s f ves _ inst (unop_error Heqves)).
-        give_up.
+        rewrite <- Heqves.
+        apply (RS''_error _ (unop_error Heqves)).
       + (* v :: ves' *)
-          Check reduce_unop.
-        apply <<hs, s, f, vs_to_es (app_unop op v :: ves')>>[
-          reduce_unop _ _ _ Heqes0
+        apply <<hs, s, f, vs_to_es (app_unop op v :: ves')>>'[
+          reduce_unop _ _ _ _ _ _ _
         ].
     * (* AI_basic (BI_binop t op) *)
       destruct ves as [|v2 [|v1 ves']] eqn:foobar.
       + (* [::] *)
-        apply (RS'_error _ _ (admitted_TODO _)).
+        apply (RS''_error _ (admitted_TODO _)).
       + (* [:: v2] *)
-        apply (RS'_error _ _ (admitted_TODO _)).
+        apply (RS''_error _ (admitted_TODO _)).
       + (* [:: v2, v1 & ves'] *)
         destruct (app_binop op v1 v2) as [v|] eqn:Heqapp.
         -- (* Some v *)
-           apply <<hs, s, f, vs_to_es (v :: ves')>>[
-             reduce_binop _ _ _ Heqes0 Heqapp
+           apply <<hs, s, f, vs_to_es (v :: ves')>>'[
+             reduce_binop _ _ _ _ _ Heqapp
            ].
         -- (* None *)
-           apply (RS'_error _ _ (admitted_TODO _)).
+           apply (RS''_error _ (admitted_TODO _)).
     * (* AI_basic (BI_testop _ testop) *) (* TODO match further *)
       give_up.
     * (* AI_basic (BI_relop t op) *)
